processor/src/DecExecOk.v
@@ -1,0 +1,367 @@
+Require Import String.
+Require Import Coq.ZArith.ZArith.
+Require Import coqutil.Z.Lia.
+Require Import Coq.Lists.List. Import ListNotations.
+Require Import Kami.Lib.Word.
+Require Import riscv.Spec.Decode.
+Require Import coqutil.Map.Interface.
+
+Require Import processor.KamiWord.
+Require Import riscv.Utility.Utility.
+
+Require Import Kami.Syntax Kami.Semantics Kami.Tactics.
+Require Import Kami.Ex.MemTypes.
+Require Import Kami.Ex.IsaRv32.
+
+Require Import processor.KamiProc.
+
+Local Open Scope Z_scope.
+
+Section DecExecOk.
+
+  Instance W: Utility.Words := @KamiWord.WordsKami width width_cases.
+
+  Variables (instrMemSizeLg: Z).
+  Hypothesis (HinstrMemBound: instrMemSizeLg <= width - 2).
+
+  Local Definition kamiProc := @KamiProc.proc instrMemSizeLg.
+  Local Definition KamiSt := @KamiProc.st instrMemSizeLg.
+
+  (** * Register file mapping *)
+
+  Context {Registers: map.map Register word}.
+
+  Definition convertRegs (rf: kword 5 -> kword width): Registers :=
+    let kkeys := HList.tuple.unfoldn (wplus (natToWord 5 1)) 31 (natToWord 5 1) in
+    let values := HList.tuple.map rf kkeys in
+    let keys := HList.tuple.map (@wordToZ 5) kkeys in
+    map.putmany_of_tuple keys values map.empty.
+
+  Lemma convertRegs_get:
+    forall rf r v,
+      map.get (convertRegs rf) (Word.wordToZ r) = Some v ->
+      v = rf r.
+  Proof.
+  Admitted.
+
+  Lemma convertRegs_put:
+    forall rf r v,
+      convertRegs (fun w => if weq w r then v else rf w) =
+      map.put (convertRegs rf) (Word.wordToZ r) v.
+  Proof.
+    intros.
+    eapply map.map_ext.
+    intros k.
+  Admitted.
+
+  Lemma invert_Kami_execNm:
+    forall km1 kt1 kupd klbl,
+      KamiProc.RegsToT km1 = Some kt1 ->
+      Step kamiProc km1 kupd klbl ->
+      klbl.(annot) = Some (Some "execNm"%string) ->
+      exists kt2: KamiSt,
+        klbl.(calls) = FMap.M.empty _ /\
+        KamiProc.RegsToT (FMap.M.union kupd km1) = Some kt2 /\
+        exists curInst npc prf dst exec_val,
+          curInst = (KamiProc.pgm kt1) (split2 _ _ (KamiProc.pc kt1)) /\
+          npc = evalExpr (rv32NextPc
+                            _ _
+                            (KamiProc.rf kt1) (KamiProc.pc kt1)
+                            curInst) /\
+          prf = KamiProc.rf kt1 /\
+          dst = evalExpr (rv32GetDst _ curInst) /\
+          exec_val = evalExpr
+                       (rv32Exec
+                          _ _
+                          (KamiProc.rf kt1 (evalExpr (rv32GetSrc1 _ curInst)))
+                          (KamiProc.rf kt1 (evalExpr (rv32GetSrc2 _ curInst)))
+                          (KamiProc.pc kt1)
+                          curInst) /\
+          kt2 = {| KamiProc.pc := npc;
+                   KamiProc.rf :=
+                     evalExpr
+                       (UpdateVector
+                          (Var _ (SyntaxKind (Vector (Bit (Z.to_nat width))
+                                                     rv32RfIdx)) prf)
+                          (Var _ (SyntaxKind (Bit rv32RfIdx)) dst)
+                          (Var _ (SyntaxKind (Bit (Z.to_nat width))) exec_val));
+                   KamiProc.pgm := KamiProc.pgm kt1;
+                   KamiProc.mem := KamiProc.mem kt1 |}.
+  Proof.
+    intros.
+    kinvert; try (repeat
+                    match goal with
+                    | [H: annot ?klbl = Some _ |- _] => rewrite H in *
+                    | [H: (_ :: _)%struct = (_ :: _)%struct |- _] =>
+                      inversion H; subst; clear H
+                    end; discriminate).
+
+    Opaque evalExpr.
+    kinv_action_dest.
+    unfold KamiProc.RegsToT in *.
+    kregmap_red.
+    destruct x1; try discriminate.
+    destruct (FMap.M.find "mem"%string km1)
+      as [[[kind|] memv]|]; try discriminate.
+    destruct (decKind kind (Vector (Bit (Z.to_nat width)) (Z.to_nat width)));
+      try discriminate.
+    kregmap_red.
+    inversion_clear H.
+    eexists; split; [|split].
+    - assumption.
+    - reflexivity.
+    - do 5 eexists.
+      repeat (split; [reflexivity|]).
+      reflexivity.
+      Transparent evalExpr.
+
+  Qed.
+
+  Ltac lets_in_hyp_to_eqs :=
+    repeat lazymatch goal with
+           | |- (let x := ?a in ?b) = ?c -> ?Q =>
+             change (let x := a in b = c -> Q); intro
+           | x := bitSlice _ 25 26 |- _ =>
+            (* shamtHi is the only field which another field depends on *)
+             subst x
+           | x := ?t : ?T |- _ =>
+             pose proof (eq_refl t : x = t); clearbody x
+           end.
+
+  Ltac invert_decode_if_true G :=
+    first [ apply Bool.andb_true_iff in G;
+            let G1 := fresh G in let G2 := fresh G in destruct G as [G1 G2];
+            invert_decode_if_true G1; invert_decode_if_true G2
+          | apply Z.eqb_eq in G
+          | idtac ].
+
+  (* TODO rather than stating this as a lemma, write a tactic which
+     infers & poses the conclusion *)
+  Lemma invert_decode_Add: forall inst rd rs1 rs2: Z,
+      decode RV32IM inst = IInstruction (Decode.Add rd rs1 rs2) ->
+      bitSlice inst 0 7 = opcode_OP /\
+      bitSlice inst 7 12 = rd /\
+      bitSlice inst 12 15 = funct3_ADD /\
+      bitSlice inst 15 20 = rs1 /\
+      bitSlice inst 20 25 = rs2 /\
+      bitSlice inst 25 32 = funct7_ADD.
+  Proof.
+    intros *.
+    cbv beta delta [decode].
+    lets_in_hyp_to_eqs.
+    subst
+      resultI
+      resultM
+      resultA
+      resultF
+      resultI64
+      resultM64
+      resultA64
+      resultF64
+      resultCSR.
+    repeat match type of H with
+    | context C [if ?a then ?b else ?c] =>
+      ((let P := context C [ b ] in change P in H) ||
+       (let P := context C [ c ] in change P in H))
+    end.
+    subst results.
+    destruct (isValidI decodeI) eqn: VI;
+    destruct (isValidM decodeM) eqn: VM;
+    destruct (isValidCSR decodeCSR) eqn: VCSR.
+    all: try (clear; simpl; discriminate).
+    simpl.
+    intro E.
+    injection E. clear E.
+    subst decodeI.
+    intro E.
+    repeat match type of E with
+    | (if ?a then ?b else ?c) = ?d => destruct a; [discriminate E|]
+    end.
+    match type of E with
+    | (if ?a then ?b else ?c) = ?d => destruct a eqn: G; cycle 1
+    end.
+    { (* more invalid cases *)
+      repeat match type of E with
+             | (if ?a then ?b else ?c) = ?d => destruct a; [discriminate E|]
+             end.
+      discriminate E.
+    }
+    (* the only valid case remains *)
+    subst rd0 rs4 rs0.
+    invert_decode_if_true G.
+    assert (bitSlice inst 0 7 = opcode_OP) as R1 by congruence; revert R1.
+    assert (bitSlice inst 12 15 = funct3_ADD) as R2 by congruence; revert R2.
+    assert (bitSlice inst 25 32 = funct7_ADD) as R3 by congruence; revert R3.
+    injection E.
+    clear.
+    (* if we automate this further, we might be able to infer the conclusion with a tactic
+       rather than having to state it manually *)
+    intros. auto.
+  Qed.
+
+  Lemma kami_split_bitSlice_consistent_1:
+    forall (i: nat) kinst,
+      wordToZ (split1 i (32 - i) kinst) =
+      bitSlice (wordToZ kinst) 0 (Z.of_nat i).
+  Proof.
+  Admitted.
+
+  Lemma kami_split_bitSlice_consistent_2:
+    forall (i j: nat) kinst,
+      wordToZ (split2 i j kinst) =
+      bitSlice (wordToZ kinst) (Z.of_nat i) (Z.of_nat (i + j)).
+  Proof.
+  Admitted.
+
+  Lemma kami_split_bitSlice_consistent_3:
+    forall (i j: nat) kinst,
+      wordToZ
+        (split2 i j (split1 (i + j) (32 - (i + j)) kinst)) =
+      bitSlice (wordToZ kinst) (Z.of_nat i) (Z.of_nat (i + j)).
+  Proof.
+  Admitted.
+
+  Lemma kami_getOpcode_ok:
+    forall kinst,
+      wordToZ
+        (evalExpr
+           (getOpcodeE (Var type (SyntaxKind (Data rv32InstBytes)) kinst))) =
+      bitSlice (wordToZ kinst) 0 7.
+  Proof.
+    intros.
+    unfold getOpcodeE.
+    unfold evalExpr; fold evalExpr.
+    unfold evalUniBit.
+    rewrite kami_split_bitSlice_consistent_1.
+    reflexivity.
+  Qed.
+
+  Lemma kami_getFunct7_ok:
+    forall kinst,
+      wordToZ
+        (evalExpr
+           (getFunct7E (Var type (SyntaxKind (Data rv32InstBytes)) kinst))) =
+      bitSlice (wordToZ kinst) 25 32.
+  Proof.
+    intros.
+    unfold getFunct7E.
+    unfold evalExpr; fold evalExpr.
+    unfold evalUniBit.
+    rewrite kami_split_bitSlice_consistent_2.
+    reflexivity.
+  Qed.
+
+  Lemma kami_getFunct3_ok:
+    forall kinst,
+      wordToZ
+        (evalExpr
+           (getFunct3E (Var type (SyntaxKind (Data rv32InstBytes)) kinst))) =
+      bitSlice (wordToZ kinst) 12 15.
+  Proof.
+    intros.
+    unfold getFunct3E.
+    unfold evalExpr; fold evalExpr.
+    unfold evalUniBit.
+    rewrite kami_split_bitSlice_consistent_3.
+    reflexivity.
+  Qed.
+
+  Lemma kami_getRdE_ok:
+    forall kinst,
+      wordToZ
+        (evalExpr (getRdE (Var type (SyntaxKind (Data rv32InstBytes)) kinst))) =
+      bitSlice (wordToZ kinst) 7 12.
+  Proof.
+    intros.
+    unfold getRdE.
+    unfold evalExpr; fold evalExpr.
+    unfold evalUniBit.
+    rewrite kami_split_bitSlice_consistent_3.
+    reflexivity.
+  Qed.
+
+  Lemma kami_rv32GetDst_ok:
+    forall kinst,
+      bitSlice (wordToZ kinst) 0 7 = opcode_OP ->
+      Word.wordToZ (evalExpr (rv32GetDst type kinst)) =
+      bitSlice (wordToZ kinst) 7 12.
+  Proof.
+    intros.
+    unfold rv32GetDst.
+    unfold evalExpr; fold evalExpr.
+    destruct (isEq _ _) as [Heq|Hne].
+    - exfalso.
+      pose proof (kami_getOpcode_ok kinst).
+      rewrite Heq, H in H0; discriminate.
+    - rewrite kami_getRdE_ok; reflexivity.
+  Qed.
+
+  Lemma kami_rv32GetSrc1_ok:
+    forall kinst,
+      Word.wordToZ (evalExpr (rv32GetSrc1 type kinst)) =
+      bitSlice (wordToZ kinst) 15 20.
+  Proof.
+    intros.
+    unfold rv32GetSrc1, getRs1E.
+    unfold evalExpr; fold evalExpr.
+    unfold evalUniBit.
+    rewrite kami_split_bitSlice_consistent_3.
+    reflexivity.
+  Qed.
+
+  Lemma kami_rv32GetSrc2_ok:
+    forall kinst,
+      Word.wordToZ (evalExpr (rv32GetSrc2 type kinst)) =
+      bitSlice (wordToZ kinst) 20 25.
+  Proof.
+    intros.
+    unfold rv32GetSrc2, getRs2E.
+    unfold evalExpr; fold evalExpr.
+    unfold evalUniBit.
+    rewrite kami_split_bitSlice_consistent_3.
+    reflexivity.
+  Qed.
+
+  (** TODO @joonwonc: ditto [invert_decode_Add]; better to have a tactic. *)
+  Lemma kami_rv32Exec_Add_ok:
+    forall v1 v2 pc kinst,
+      wordToZ
+        (evalExpr
+           (getOpcodeE (Var type (SyntaxKind (Data rv32InstBytes)) kinst))) =
+      opcode_OP ->
+      wordToZ
+        (evalExpr (getFunct7E (Var type (SyntaxKind (Data rv32InstBytes)) kinst))) =
+      funct7_ADD ->
+      wordToZ
+        (evalExpr (getFunct3E (Var type (SyntaxKind (Data rv32InstBytes)) kinst))) =
+      funct3_ADD ->
+      evalExpr (rv32Exec (Z.to_nat instrMemSizeLg) type v1 v2 pc kinst) =
+      v1 ^+ v2.
+  Proof.
+    intros.
+    unfold rv32Exec.
+    unfold evalExpr; fold evalExpr.
+    do 5 (destruct (isEq _ _); [rewrite e in H; discriminate|clear n]).
+    do 3 (destruct (isEq _ _); [|exfalso; elim n; apply wordToZ_inj; assumption]).
+    reflexivity.
+  Qed.
+
+  Lemma kami_rv32NextPc_op_ok:
+    forall rf pc kinst,
+      wordToZ
+        (evalExpr
+           (getOpcodeE (Var type (SyntaxKind (Data rv32InstBytes)) kinst))) =
+      opcode_OP ->
+      evalExpr (rv32NextPc (Z.to_nat instrMemSizeLg) type rf pc kinst) =
+      pc ^+ $4.
+  Proof.
+    intros.
+    unfold rv32NextPc.
+    unfold evalExpr; fold evalExpr.
+    do 3 (destruct (isEq _ _); [rewrite e in H; discriminate|clear n]).
+    unfold evalBinBit.
+    unfold evalConstT.
+    f_equal.
+  Admitted.
+
+End DecExecOk.
