processor/src/FetchOk.v
@@ -1,0 +1,93 @@
+Require Import String.
+Require Import Coq.ZArith.ZArith.
+Require Import coqutil.Z.Lia.
+Require Import Coq.Lists.List. Import ListNotations.
+Require Import Kami.Lib.Word.
+Require Import coqutil.Word.LittleEndian.
+Require Import coqutil.Map.Interface.
+
+(* In order to just use [word] as a typeclass [processor.KamiWord] should
+ * be imported before importing [riscv.Utility.Utility]. *)
+Require Import processor.KamiWord.
+Require Import riscv.Utility.Utility.
+
+Require riscv.Platform.Memory.
+Require Import riscv.Platform.RiscvMachine.
+
+Require Import processor.KamiProc.
+
+Local Open Scope Z_scope.
+
+Section FetchOk.
+
+  Instance W: Utility.Words := @KamiWord.WordsKami width width_cases.
+  Context {mem: map.map word byte}.
+
+  (* [instrMemSizeLg] is the log number of instructions in the instruction cache.
+   * If the instruction base address is just 0, then the address range for
+   * the instructions is [0 -- 4 * 2^(instrMemSizeLg)].
+   *)
+  Variable instrMemSizeLg: Z.
+  Hypothesis (HinstrMemBound: instrMemSizeLg <= width - 2).
+  Definition instrMemSize: nat := Z.to_nat (Z.pow 2 instrMemSizeLg).
+  Definition instrMemStart: kword instrMemSizeLg := Word.ZToWord _ 0.
+  Definition instrMemStart': word := Word.ZToWord _ 0.
+
+  Variable dataMemSize: nat.
+  Definition dataMemStart: word := word.of_Z (Z.of_nat (4 * instrMemSize)).
+
+  Definition word32_to_4bytes (w: kword 32): HList.tuple byte 4 :=
+    LittleEndian.split 4 (word.unsigned w).
+
+  (* TODO this structure might not be very proof friendly, 
+   * use Memory.unchecked_store_byte_list instead *)
+  Fixpoint unchecked_store_byte_tuple_list{n: nat}(a: word)(l: list (HList.tuple byte n))(m: mem): mem :=
+    match l with
+    | w :: rest =>
+      let m' := unchecked_store_byte_tuple_list (word.add a (word.of_Z (Z.of_nat n))) rest m in
+      Memory.unchecked_store_bytes n m' a w
+    | nil => m
+    end.
+
+  (* set of executable addresses in the kami processor *)
+  Definition kamiXAddrs: XAddrs := addXAddrRange instrMemStart' instrMemSize nil.
+
+  Definition convertInstrMem (instrMem: kword instrMemSizeLg -> kword 32): mem :=
+    let keys := List.unfoldn (Word.wplus (Word.ZToWord (Z.to_nat instrMemSizeLg) 1))
+                             instrMemSize instrMemStart in
+    let values := List.map (fun key => word32_to_4bytes (instrMem key)) keys in
+    @unchecked_store_byte_tuple_list 4 (word.of_Z 0) values map.empty.
+
+  Definition convertDataMem(dataMem: kword width -> kword width): mem :=
+    let keys := List.unfoldn (word.add (word.of_Z (width / 8))) dataMemSize dataMemStart in
+    let values := List.map (fun key => LittleEndian.split (Z.to_nat (width / 8))
+                                                          (word.unsigned (dataMem key)))
+                           keys in
+    unchecked_store_byte_tuple_list dataMemStart values map.empty.
+
+  Definition toKamiPc (pc: kword width):
+    Word.word (2 + Z.to_nat instrMemSizeLg) :=
+    $(#pc).
+
+  Lemma toKamiPc_wplus_distr:
+    forall w1 w2,
+      toKamiPc w1 ^+ toKamiPc w2 = toKamiPc (w1 ^+ w2).
+  Proof.
+  Admitted.
+
+  Lemma fetch_ok:
+    forall (instrMem: kword instrMemSizeLg -> kword width)
+           (dataMem: kword width -> kword width)
+           (pc: kword width),
+      isXAddr pc kamiXAddrs ->
+      exists (inst: HList.tuple byte 4),
+        Memory.loadWord
+          (map.putmany (convertInstrMem instrMem)
+                       (convertDataMem dataMem)) pc = Some inst /\
+        combine 4 inst =
+        wordToZ (instrMem
+                   (split2 2 (Z.to_nat instrMemSizeLg) (toKamiPc pc))).
+  Proof.
+  Admitted.
+
+End FetchOk.
